src/DiscreteMemory.v
@@ -1,0 +1,742 @@
+Require Import Heaps.
+Require Import Setoid.
+Require Import DepList.
+Require Import List.
+
+Module Type DiscreteMemory.
+  Parameter addr : Type.
+  
+  Parameter all_addr : list addr.
+  
+  Parameter NoDup_all_addr : NoDup all_addr.
+End DiscreteMemory.
+
+(** A permission-like view on top of concrete memories **)
+Module DiscreteHeap (B : Memory)
+                    (BD : DiscreteMemory with Definition addr := B.addr) 
+                 <: SeparationMemory with Module M := B.
+  Module Import M := B.
+
+  Instance EqDec_addr : EquivDec.EqDec addr (@eq addr) := addr_dec.
+
+  Definition smem' dom : Type := hlist (fun _ : addr => option value) dom.
+
+  Fixpoint smem_emp' (ls : list addr) : smem' ls :=
+    match ls with
+      | nil => HNil
+      | a :: b => HCons None (smem_emp' b)
+    end.
+  Fixpoint disjoint' dom : smem' dom -> smem' dom -> Prop :=
+    match dom with
+      | nil => fun _ _ => True
+      | a :: b => fun m1 m2 => 
+           (hlist_hd m1 = None \/ hlist_hd m2 = None) 
+        /\ disjoint' _ (hlist_tl m1) (hlist_tl m2)
+    end.
+  Fixpoint join' dom : smem' dom -> smem' dom -> smem' dom :=
+    match dom with
+      | nil => fun _ _ => HNil
+      | a :: b => fun m1 m2 => 
+        HCons 
+        match hlist_hd m1 with
+          | None => hlist_hd m2
+          | Some x => Some x
+        end
+        (join' _ (hlist_tl m1) (hlist_tl m2))
+    end.
+
+  Fixpoint relevant' (ls : list addr) : smem' ls -> list addr :=
+    match ls with
+      | nil => fun _ => nil
+      | a :: b => fun x => 
+        match hlist_hd x with
+          | None => relevant' _ (hlist_tl x)
+          | Some _ => a :: relevant' _ (hlist_tl x)
+        end
+    end.
+  
+  Fixpoint smem_get' dom : addr -> smem' dom -> option value :=
+    match dom as dom return addr -> smem' dom -> option value with 
+      | nil => fun _ _ => None
+      | a :: b => fun a' m =>
+        if addr_dec a a' then 
+          hlist_hd m
+        else
+          smem_get' b a' (hlist_tl m)
+    end.
+
+  Fixpoint smem_set' dom : addr -> value -> smem' dom -> option (smem' dom) :=
+    match dom as dom return addr -> value -> smem' dom -> option (smem' dom) with 
+      | nil => fun _ _ _ => None
+      | a :: b => fun p v m =>
+        if addr_dec a p then
+          match hlist_hd m with
+            | None => None
+            | Some _ => Some (HCons (Some v) (hlist_tl m))
+          end
+        else
+          match smem_set' b p v (hlist_tl m) with
+            | None => None
+            | Some tl => Some (HCons (hlist_hd m) tl)
+          end
+    end.
+
+  Fixpoint models' dom (sm : smem' dom) (m : B.mem) : Prop :=
+    match sm with
+      | HNil => True
+      | HCons p _ a b =>
+        match a with
+          | None => True
+          | Some x => 
+            B.mem_get m p = Some x
+        end /\ models' _ b m
+    end.
+
+  Definition smem : Type := smem' BD.all_addr.
+
+  Definition smem_eqv : smem -> smem -> Prop := @eq smem.
+
+  Definition smem_emp : smem := smem_emp' BD.all_addr.
+
+  Definition smem_get := @smem_get' BD.all_addr.
+
+  Definition smem_set := @smem_set' BD.all_addr.
+
+  Definition disjoint (m1 m2 : smem) : Prop :=
+    disjoint' _ m1 m2.
+
+  Definition join (m1 m2 : smem) : smem := 
+    join' _ m1 m2.
+
+  Definition split (m ml mr : smem) : Prop :=
+    disjoint ml mr /\ m = join ml mr.
+
+  Definition semp (m : smem) : Prop :=
+    m = smem_emp.
+
+  Definition models (m : smem) (m' : B.mem) : Prop :=
+    models' _ m m'.
+(*
+  Definition relevant (sm : smem) := relevant' _ sm.
+*)
+
+  Theorem Reflexive_eqv : Reflexive smem_eqv.
+  Proof. intuition. Qed.
+
+  Theorem Symmetric_eqv : Symmetric smem_eqv.
+  Proof. intuition. Qed.
+
+  Theorem Transitive_eqv : Transitive smem_eqv.
+  Proof. unfold smem_eqv; intuition. Qed.
+
+  Theorem models_respects : forall s s' m,
+    smem_eqv s s' ->
+    (models s m <-> models s' m).
+  Proof. unfold smem_eqv; intuition subst; auto. Qed.
+ 
+  Theorem smem_get_respects : forall a s s',
+    smem_eqv s s' -> smem_get a s = smem_get a s'.
+  Proof. unfold smem_eqv; intuition subst; auto. Qed.    
+
+  Theorem smem_set_respects : forall a v s s',
+    smem_eqv s s' -> smem_set a v s = smem_set a v s'.
+  Proof. unfold smem_eqv; intuition subst; auto. Qed.    
+
+  Theorem split_respects : forall s1 s1' s2 s2' s3 s3',
+    smem_eqv s1 s1' -> smem_eqv s2 s2' -> smem_eqv s3 s3' ->
+    (split s1 s2 s3 <-> split s1' s2' s3').
+  Proof. unfold smem_eqv; intuition subst; auto. Qed.
+
+  Theorem split_emp : forall a c,
+    split a smem_emp c <-> smem_eqv a c.
+  Proof.
+    unfold split, smem_emp, smem_eqv, disjoint, join, smem.
+    generalize dependent BD.all_addr.
+    induction l; simpl in *; intros.
+    { intuition; subst; auto; rewrite hlist_nil_only with (h := c); eauto with typeclass_instances. }
+    { intuition subst; rewrite hlist_eta with (h := c); eauto with typeclass_instances; f_equal;
+      eapply IHl; intuition. }
+  Qed.
+ 
+  Theorem split_comm : forall a b c,
+    split a b c -> split a c b.
+  Proof. 
+    unfold split, join, disjoint, smem.
+    generalize dependent BD.all_addr.
+    induction l; simpl in *; intros; auto.
+    destruct H. destruct H. subst.
+    destruct (IHl _ _ _ (conj H1 eq_refl)). 
+    rewrite H2. intuition; rewrite H3; try f_equal.
+    destruct (hlist_hd c); auto.
+    destruct (hlist_hd b); auto.
+  Qed.
+
+  Theorem split_assoc : forall a b c d e,
+    split a b c -> split b d e ->
+    exists f, split a d f /\ split f e c.
+  Proof.
+    unfold split, join, disjoint, smem.
+    generalize dependent BD.all_addr.
+    induction l; simpl in *; intros; auto.
+    { intuition subst. exists HNil; intuition. }
+    { repeat match goal with
+               | [ H : _ /\ _ |- _ ] => destruct H
+               | [ H : _ = _ |- _ ] => rewrite H
+             end; subst; simpl in *.
+      destruct (IHl _ _ _ _ _ (conj H4 eq_refl) (conj H2 eq_refl)); clear IHl.
+      repeat match goal with
+               | [ H : _ /\ _ |- _ ] => destruct H
+               | [ H : _ = _ |- _ ] => rewrite H
+             end; subst; simpl in *.
+      intuition; eexists; intuition; repeat match goal with
+                          | [ H : _ /\ _ |- _ ] => destruct H
+                          | [ H : _ = _ |- _ ] => rewrite H in *
+                        end; subst; simpl in *; eauto.
+      destruct (hlist_hd d); auto.
+      destruct (hlist_hd d); auto; try congruence.
+      destruct (hlist_hd d); auto. }
+  Qed.
+
+  Theorem smem_get_sound : forall s m,
+    models s m ->
+    forall a v, smem_get a s = Some v ->
+                M.mem_get m a = Some v.
+  Proof.
+  Admitted.
+
+  Theorem smem_set_sound : forall s m,
+    models s m ->
+    forall a v s', smem_set a v s = Some s' ->
+    exists m', M.mem_set m a v = Some m' /\ models s' m'. 
+  Proof.
+  Admitted.
+
+  (** memoryIn **)
+  Section memoryIn.
+    Variable m : mem.
+
+    Fixpoint memoryIn' (ls : list addr) : smem' ls :=
+      match ls with 
+        | nil => HNil
+        | l :: ls => HCons (mem_get m l) (memoryIn' ls)
+      end. 
+
+    Definition memoryIn : smem := memoryIn' BD.all_addr.
+  End memoryIn.
+
+  Theorem memoryIn_sound : forall m, 
+    models (memoryIn m) m.
+  Proof.
+    unfold models, memoryIn. generalize BD.all_addr.
+    induction l; simpl; auto.
+    intuition. destruct (mem_get m a); auto.
+  Qed.
+
+End DiscreteHeap.
+
+Export Heaps.
+
+(*
+  Local Hint Resolve mem_get_set_eq mem_get_set_neq : memory.
+
+  Lemma smem_set_not_in : forall l m p v,
+    ~In p l -> smem_set' l p v m = None.
+  Proof.
+    induction l; simpl; auto.
+      intros.
+      destruct (addr_dec a p); subst; intuition.
+      rewrite IHl; auto.
+  Qed.
+
+  Ltac simp ext :=
+    intros; simpl in *;
+    repeat (instantiate; 
+      match goal with
+        | [ H : prod _ _ |- _ ] => destruct H
+        | [ H : Some _ = Some _ |- _ ] =>
+          inversion H; clear H; try subst
+        | [ H : _ = _ |- _ ] => rewrite H in *
+        | [ H : NoDup (_ :: _) |- _ ] =>
+          inversion H; clear H; subst
+        | [ H : context [ addr_dec ?A ?B ] |- _ ] => 
+          destruct (addr_dec A B); subst
+        | [ |- context [ addr_dec ?A ?B ] ] => 
+          destruct (addr_dec A B); subst
+        | [ H : match ?X with 
+                  | Some _ => _
+                  | None => _
+                end = _ |- _ ] => 
+          generalize dependent H; case_eq X; intros
+        | [ H : match ?X with 
+                  | Some _ => _
+                  | None => _
+                end |- _ ] => 
+          generalize dependent H; case_eq X; intros
+        | [ H : models' (_ :: _) ?M _ |- _ ] =>
+          match M with
+            | HCons _ _ => fail 1
+            | _ => rewrite (hlist_eta _ M) in H
+          end
+        | [ |- models' (_ :: _) ?M _ ] =>
+          match M with
+            | HCons _ _ => fail 1
+            | _ => rewrite (hlist_eta _ M)
+          end
+        | [ H : smem' nil |- _ ] => 
+          rewrite (hlist_nil_only _ H) in *
+        | [ H : exists x, _ |- _ ] => destruct H
+        | [ H : _ /\ _ |- _ ] => destruct H
+        | [ |- _ ] => congruence
+        | [ |- _ ] => ext
+      end; simpl in * ); eauto 10 with memory.
+
+  Theorem satisfies_get : forall m m',
+    models m m' ->
+    forall p v, 
+      smem_get p m = Some v ->
+      mem_get m' p = Some v.
+  Proof.
+    unfold models, smem_get, smem.
+    induction BD.all_addr; simp intuition. 
+  Qed.
+
+  Lemma models_set_not_in : forall l m sm p v,
+    models' l sm m ->
+    ~In p l ->
+    forall m', mem_set m p v = Some m' ->
+    models' l sm m'.
+  Proof.
+    induction l; try solve [ simp intuition ].
+      simp auto.
+      destruct (addr_dec a p); destruct (in_dec addr_dec p l); subst; try solve [ intuition ].
+
+      split; eauto. rewrite <- H3. eapply B.mem_get_set_neq; eauto.
+  Qed.
+
+  Local Hint Resolve models_set_not_in : memory.
+
+  Theorem models_set : forall sm m,
+    models sm m ->
+    forall p v sm',
+      smem_set p v sm = Some sm' ->
+      exists m',
+      mem_set m p v = Some m' /\ models sm' m'.
+  Proof.
+    unfold models, smem_set, smem_get, smem.
+    generalize BD.NoDup_all_addr.
+    induction BD.all_addr; simp auto.
+    { 
+
+
+      destruct (proj1 (mem_set_acc _ _) H2 v). rewrite H3. eexists; split; eauto.        
+      erewrite mem_get_set_eq; eauto with memory.
+
+      Focus.
+      eapply IHl in H1; eauto.
+      destruct H1; eexists; intuition; eauto with memory.
+      erewrite mem_get_set_neq; eauto.
+
+      Focus.
+      eapply IHl in H1; eauto. destruct H1; eexists; intuition eauto.
+  Qed.
+
+  Lemma smem_set_get_neq : forall p m m' a b,
+    smem_set a b m = Some m' ->
+    a <> p ->
+    smem_get p m' = smem_get p m.
+  Proof.
+    unfold smem, smem_get, smem_set.
+    induction BD.all_addr; simp intuition.
+  Qed.
+
+  Lemma smem_set_get_eq : forall m m' a b,
+    smem_set a b m = Some m' ->
+    smem_get a m' = Some b.
+  Proof.
+    unfold smem, smem_get, smem_set.
+    induction BD.all_addr; simp intuition.
+  Qed.
+
+  Lemma split_smem_get : forall a b c p v,
+    split a b c ->
+      (smem_get p b = Some v \/ smem_get p c = Some v) ->
+      smem_get p a = Some v.
+  Proof.
+    unfold smem, split, disjoint, join, smem_get, smem.
+    induction BD.all_addr; simp intuition.
+  Qed.
+
+  Lemma smem_set_get_valid : forall m p v v',
+    smem_get p m = Some v' ->
+    smem_set p v m <> None.
+  Proof.
+    unfold smem_get, smem_set, smem.
+    induction BD.all_addr; simp intuition.
+  Qed.
+
+  Lemma split_set : forall a b,
+    disjoint a b ->
+    forall p v a',
+    smem_set p v a = Some a' ->
+      disjoint a' b /\ 
+      smem_set p v (join a b) = Some (join a' b).
+  Proof.
+    unfold smem, disjoint, join, smem_set, smem.
+    induction BD.all_addr; simpl; intros; try congruence.
+      destruct (addr_dec a p); subst.
+      destruct H. destruct H; rewrite H in *; try congruence.
+        destruct (hlist_hd a0); try congruence.
+        inversion H0; auto.
+
+      generalize dependent H0.
+      case_eq (smem_set' l p v (hlist_tl a0)); intros; try congruence.
+        inversion H1; clear H1; subst.
+        eapply IHl in H0. 2: destruct H; eauto.
+        simp intuition.
+  Qed.
+
+
+  Ltac unfold_all :=
+    unfold smem, split, join, disjoint, smem_emp, semp; 
+    unfold smem, split, join, disjoint, smem_emp, semp.
+  Ltac break :=
+    simpl; intros; try reflexivity;
+      repeat (simpl in *; match goal with
+                            | [ H : HCons _ _ = HCons _ _ |- _ ] =>
+                              inversion H; clear H
+                            | [ H : _ /\ _ |- _ ] => destruct H
+                            | [ H : @existT _ _ _ _ = @existT _ _ _ _ |- _ ] => 
+                              eapply (@Eqdep_dec.inj_pair2_eq_dec _ (list_eq_dec B.addr_dec)) in H
+                            | [ H : @existT _ _ _ _ = @existT _ _ _ _ |- _ ] => 
+                              eapply (@Eqdep_dec.inj_pair2_eq_dec _ B.addr_dec) in H
+                            | [ H : _ = _ |- _ ] => rewrite H in *
+                          end).
+  
+  Lemma disjoint_join : forall a b, disjoint a b -> join a b = join b a.
+  Proof.
+    unfold_all; induction a; break; f_equal; intuition; subst.
+      destruct (hlist_hd b0); reflexivity.
+      rewrite H1. destruct b; reflexivity.
+  Qed.
+    
+  Lemma disjoint_comm : forall ml mr, disjoint ml mr -> disjoint mr ml.
+  Proof.
+    unfold_all; induction ml; break; intuition.
+  Qed.
+
+  Hint Resolve disjoint_join disjoint_comm : disjoint.
+
+  Lemma split_assoc' : forall b a c d e, split a b c -> split c d e ->
+    split a (join d b) e.
+  Proof.
+    unfold_all; induction b; break; eauto.
+    edestruct IHb. split; try eassumption. reflexivity. split; try eassumption.
+    reflexivity.
+    intuition; break; auto. destruct (hlist_hd d); auto.
+    destruct (hlist_hd d); try congruence.
+  Qed.
+
+  Lemma split_comm : forall m ml mr, split m ml mr -> split m mr ml.
+  Proof.
+    unfold_all. induction ml; break; eauto. edestruct IHml.
+    split; try eassumption. reflexivity. 
+    intuition; subst. rewrite H3. destruct (hlist_hd mr); auto.
+    rewrite H4. rewrite H3. destruct b; auto.
+  Qed.
+
+  Lemma disjoint_split_join : forall a b, disjoint a b -> split (join a b) a b.
+  Proof.
+    unfold split, disjoint; intros; intuition.
+  Qed.
+
+  Lemma split_split_disjoint : forall b a c d e,
+    split a b c -> split b d e -> disjoint c d.
+  Proof.
+    unfold_all. induction b; break. subst. split.
+    intuition; destruct (hlist_hd c); eauto. destruct (hlist_hd d); auto.
+    eapply IHb. split; auto. split; auto. auto.
+  Qed.
+
+  Lemma hlist_destruct : forall T (F : T -> Type) a b (m : hlist F (a :: b)),
+    exists A, exists B, m = HCons A B.
+  Proof.
+    intros.
+    refine (match m as m in hlist _ ls return
+              match ls as ls return hlist _ ls -> Type with
+                | nil => fun _ => unit
+                | a :: b => fun m => exists A : F a, exists B : hlist F b, m = HCons A B
+              end m
+              with
+              | HNil => tt
+              | HCons _ _ _ _ => _
+            end).
+    do 2 eexists; reflexivity.
+  Qed.
+  Lemma hlist_nil : forall T (F : T -> Type) (m : hlist F nil), m = HNil.
+  Proof.
+    intros. 
+    refine (match m as m in hlist _ ls return
+              match ls as ls return hlist _ ls -> Type with
+                | nil => fun m => m = HNil
+                | _ :: _ => fun _ => unit
+              end m
+              with
+              | HNil => _ 
+              | _ => tt
+            end). reflexivity.
+  Qed.
+
+  Lemma split_semp : forall b a c, 
+    split a b c -> semp b -> a = c.
+  Proof.
+    unfold_all. unfold semp, smem_emp. unfold_all.
+    induction b; simpl; intros; subst; auto.
+    rewrite hlist_nil. rewrite (hlist_nil _ _ a). reflexivity.
+    destruct (hlist_destruct _ _ _ _ a).
+    destruct (hlist_destruct _ _ _ _ c).
+    destruct H1. destruct H2. subst. specialize (IHb x2 x3).
+    rewrite IHb; break; intuition; auto.
+  Qed.
+
+  Lemma semp_smem_emp : semp smem_emp.
+  Proof.
+    unfold semp, smem_emp; auto.
+  Qed.
+
+  Lemma split_a_semp_a : forall a, 
+    split a smem_emp a.
+  Proof.
+    unfold_all. induction a; simpl; intuition. rewrite <- H0. reflexivity.
+  Qed.
+     
+  Lemma cons_not_in : forall T (a : T) b ls,
+    a :: b = ls ->
+    ~ In a ls ->
+    forall P, P.
+  Proof.
+    intros; subst. exfalso; eapply H0. firstorder.
+  Qed.
+  
+  Lemma relevant_in : forall a l b,
+    In a (relevant' l b) ->
+    In a l.
+  Proof.
+    induction l; auto; intros.
+      rewrite (hlist_eta _ b) in H. simpl in H.
+      destruct (hlist_hd b). destruct H. subst. firstorder.
+      simpl in *. right. eapply IHl; eauto.
+      right. eapply IHl; eauto.
+  Qed.
+
+  Lemma relevant_not_in : forall a l b,
+    ~In a l ->
+    ~In a (relevant' l b).
+  Proof.
+    intros. intro. eapply H. eapply relevant_in; eauto.
+  Qed.
+
+  Lemma relevant_eq : forall a b c,
+    relevant a = relevant b ->
+    models a c ->
+    models b c ->
+    a = b.
+  Proof.
+    unfold relevant, models, smem. generalize BD.NoDup_all_addr.
+    induction BD.all_addr; simpl; intros.
+      rewrite (hlist_nil_only _ a). rewrite (hlist_nil_only _ b); auto.
+
+      rewrite (hlist_eta _ a0) in *. rewrite (hlist_eta _ a0) in H1.
+      rewrite (hlist_eta _ b) in *. rewrite (hlist_eta _ b) in H2.
+      simpl in *.
+      destruct (hlist_hd a0); destruct (hlist_hd b); intuition.
+        rewrite H2 in H3. inversion H3; subst. inversion H0;  f_equal. eapply IHl; eauto.
+          inversion H; auto.
+
+        eapply cons_not_in. eassumption.
+        eapply relevant_not_in. inversion H; auto.
+
+        eapply cons_not_in. symmetry. eassumption.
+        eapply relevant_not_in. inversion H; auto.
+        
+        f_equal; eauto. inversion H. eapply IHl; eauto.
+  Qed.
+
+  (** memoryIn **)
+  Section memoryIn.
+    Variable m : mem.
+
+    Fixpoint memoryIn' (ls : list addr) : smem' ls :=
+      match ls with 
+        | nil => HNil
+        | l :: ls => HCons (mem_get m l) (memoryIn' ls)
+      end. 
+
+    Definition memoryIn : smem := memoryIn' BD.all_addr.
+  End memoryIn.
+
+  Theorem smem_set_relevant : forall p v sm sm',
+    smem_set p v sm = Some sm' ->
+    relevant sm = relevant sm'.
+  Proof.
+    unfold relevant, smem_set.
+    induction BD.all_addr; simpl; intros; auto.
+      destruct (addr_dec a p); subst; auto.
+      destruct (hlist_hd sm); try congruence.
+      inversion H; clear H; subst. simpl. reflexivity.
+
+      revert H. case_eq (smem_set' l p v (hlist_tl sm)); intros; try congruence.
+      inversion H0; clear H0; subst; simpl in *.
+      destruct (hlist_hd sm); eauto. f_equal; eauto.
+  Qed.
+
+
+  Theorem models_memoryIn : forall m, 
+    models (memoryIn m) m.
+  Proof.
+    unfold models, memoryIn. generalize BD.all_addr.
+    induction l; simpl; auto.
+    intuition. destruct (mem_acc_dec m a).
+    generalize (proj1 (mem_get_acc _ _) H). intro. destruct H0. rewrite H0. auto.
+    case_eq (mem_get m a); intuition; auto.
+    eapply mem_get_acc. eauto.
+  Qed.
+
+  
+
+
+
+(*
+  Theorem smem_set_word_relevant : forall ex p v sm sm',
+    smem_set_word ex p v sm = Some sm' ->
+    relevant sm = relevant sm'.
+  Proof.
+    unfold smem_set_word; intros.
+    destruct (footprint_w p) as [ [ [ ? ? ] ? ] ? ].
+    destruct (ex v) as [ [ [ ? ? ] ? ] ? ].
+    repeat match goal with
+             | [ H : match ?X with 
+                       | Some _ => _
+                       | None => _ 
+                     end = Some _ |- _ ] => revert H; case_eq X; intros; try congruence
+             | [ H : smem_set _ _ _ = Some _ |- _ ] => 
+               eapply smem_set_relevant in H
+           end.
+    congruence.
+  Qed.
+*)
+
+
+(*
+  Definition smem_get_word (implode : B * B * B * B -> W) (p : addr) (m : smem)
+    : option W :=
+    let '(a,b,c,d) := footprint_w p in
+    match smem_get a m , smem_get b m , smem_get c m , smem_get d m with
+      | Some a , Some b , Some c , Some d =>
+        Some (implode (a,b,c,d))
+      | _ , _ , _ , _ => None
+    end.
+
+  Definition smem_set_word (explode : W -> B * B * B * B) (p : addr) (v : W)
+    (m : smem) : option smem :=
+    let '(a,b,c,d) := footprint_w p in
+    let '(av,bv,cv,dv) := explode v in
+    match smem_set d dv m with
+      | None => None 
+      | Some m => match smem_set c cv m with
+                    | None => None
+                    | Some m => match smem_set b bv m with
+                                  | None => None
+                                  | Some m => smem_set a av m
+                                end
+                  end
+    end.
+*)
+
+(*
+  Lemma split_set_word : forall a b,
+    disjoint a b ->
+    forall i p v a',
+    smem_set_word i p v a = Some a' ->
+      disjoint a' b /\ 
+      smem_set_word i p v (join a b) = Some (join a' b).
+  Proof.
+    unfold smem_set_word.
+    intros. destruct (i v); simp fail. 
+    repeat match goal with
+      | [ H : smem_set _ _ _ = Some _ |- _ ] =>
+        eapply split_set in H; [ rewrite (proj2 H) | eauto ]
+    end; tauto.
+  Qed.
+*)
+
+
+(*
+  Lemma smem_set_get_word_eq : forall i e m m' a b,
+    (forall x, i (e x) = x) ->
+    smem_set_word e a b m = Some m' ->
+    smem_get_word i a m' = Some b.
+  Proof.
+    unfold smem_get_word, smem_set_word; intros.
+    generalize (footprint_disjoint a).
+    generalize dependent H0. case_eq (e b). simp intuition.
+    specialize (H2 _ _ _ _ (refl_equal _)). simp intuition.
+    repeat ((erewrite smem_set_get_eq; [ | repeat rewrite smem_set_get_neq by auto; eassumption ])
+      || (erewrite smem_set_get_neq by eauto)). simp intuition.
+  Qed.
+*)
+
+(*
+  Lemma split_smem_get_word : forall i a b c p v,
+    split a b c ->
+      (smem_get_word i p b = Some v \/ smem_get_word i p c = Some v) ->
+      smem_get_word i p a = Some v.
+  Proof.
+    unfold smem_get_word. simp intuition;
+    repeat (erewrite split_smem_get by eauto); auto.
+  Qed.
+
+  Theorem models_set_word : forall sm m,
+    models sm m ->
+    forall e p v sm',
+      smem_set_word e p v sm = Some sm' ->
+      exists m',
+           mem_set_word addr mem footprint_w mem_set e p v m = Some m' 
+        /\ models sm' m'.
+  Proof.
+    unfold smem_set_word, mem_set_word, smem_get_word; intros.
+    simp intuition. destruct (e v); simp intuition.
+    repeat match goal with
+             | [ H : models _ _ |- _ ] => 
+               eapply models_set in H; eauto; destruct H as [ ? [ ? ? ] ]
+             | [ H : _ = _ |- _ ] => rewrite H
+           end.
+    exists x2. intuition eauto.
+  Qed.
+*)
+
+(*
+  Lemma smem_set_get_valid_word : forall i e m p v v',
+    smem_get_word i p m = Some v' ->
+    smem_set_word e p v m <> None.
+  Proof.
+    unfold smem_get_word, smem_set_word.
+    intros. generalize (footprint_disjoint p).
+    intros; destruct (e v); simp intuition;
+    specialize (H0 _ _ _ _ (refl_equal _)); simp intuition;
+    (eapply smem_set_get_valid; [ | eauto ];
+      repeat (erewrite smem_set_get_neq; [ | solve [ eauto ] | solve [ eauto ] ]); eauto).
+  Qed.
+*)
+
+(*
+  Theorem models_get_word : forall i m m',
+    models m m' ->
+    forall p v, 
+      smem_get_word i p m = Some v ->
+      mem_get_word addr mem footprint_w mem_get i p m' = Some v.
+  Proof.
+    unfold mem_get_word, smem_get_word; simp intuition.
+    repeat erewrite models_get by eauto. auto.
+  Qed.
+*)
+*)
